pancake/semantics/panSemScript.sml
@@ -117,9 +117,13 @@ Termination
 End
 
 Definition pan_op_def:
-  pan_op Div [w1;w2] = SOME(w1 / w2) ∧
+  (pan_op Div [w1;w2] =
+   if w2 ≠ 0w then SOME(w1 / w2)
+   else NONE) ∧
   pan_op Mul [w1;w2] = SOME(w1 * w2) ∧
-  pan_op Mod [w1;w2] = SOME(word_mod w1 w2) ∧
+  (pan_op Mod [w1;w2] =
+   if w2 ≠ 0w then SOME(word_mod w1 w2)
+   else NONE) ∧
   pan_op _ _ = NONE
 End
 
